

A31. f)

$$\Phi(t) = A_d(t) = \sum_{n=0}^{+\infty} \frac{A_c^n t^n}{n!} ; B_d(t) = \sum_{n=0}^{+\infty} \frac{A_c^n t^{n+1}}{(n+1)!} B_c$$

$$X(k+1) = A_d(t) X(k) + B_d(t) u(k); u(k) \text{ hat } \frac{T}{2} \text{ Verzögerung}$$

benutzen: u_{previous} $k^T X(k)$ $X(k+1)$

$$X(k+1) = A_d(\frac{T}{2}) X(k+\frac{1}{2}) + B_d(\frac{T}{2}) k^T X(k)$$

$$X(k+\frac{1}{2}) = A_d(\frac{T}{2}) X(k) + B_d(\frac{T}{2}) u(\text{previous})$$

$$Z(k) = \begin{pmatrix} X(k) \\ u(\text{previous}) \end{pmatrix}; Z(k+1) = \begin{pmatrix} X(k+1) \\ u(\text{current}) \end{pmatrix} \quad u_{\text{current}} = u(k); u_{\text{previous}} = u(k-1)$$

$$X(k+1) = A_d^2(\frac{T}{2}) X(k) + A_d(\frac{T}{2}) B_d(\frac{T}{2}) u(k-1) + B_d(\frac{T}{2}) k^T X(k)$$

$$X(k+1) = (A_d^2(\frac{T}{2}) + B_d(\frac{T}{2}) k^T) X(k) + A_d(\frac{T}{2}) B_d(\frac{T}{2}) u(k-1)$$

$$u(k) = k^T X(k)$$

$$\Rightarrow \begin{pmatrix} X(k+1) \\ u(k) \end{pmatrix} = \begin{pmatrix} A_d^2(\frac{T}{2}) + B_d(\frac{T}{2}) k^T & A_d(\frac{T}{2}) B_d(\frac{T}{2}) \\ k^T & 0 \end{pmatrix} \begin{pmatrix} X(k) \\ u(k) \end{pmatrix}$$

$$k^T = \begin{pmatrix} -\frac{1}{4} & -\frac{7}{8} \end{pmatrix}; A_c = \begin{pmatrix} 0 & 1 \\ 0 & 0 \end{pmatrix}; B_c = \begin{pmatrix} 0 \\ 1 \end{pmatrix}$$

$$A_c^2 = \begin{pmatrix} 0 & 1 \\ 0 & 0 \end{pmatrix} \begin{pmatrix} 0 & 1 \\ 0 & 0 \end{pmatrix} = \begin{pmatrix} 0 & 0 \\ 0 & 0 \end{pmatrix}$$

$$\Rightarrow A_d(t=\frac{T}{2}) = \sum_{n=0}^{+1} \frac{A_c^n (\frac{T}{2})^n}{n!} = I_{2 \times 2} + A_c^1 (\frac{T}{2})^1 = \begin{pmatrix} 1 & \frac{T}{2} \\ 0 & 1 \end{pmatrix}$$

$$B_d(t=\frac{T}{2}) = \sum_{n=0}^{+1} \frac{A_c^n t^{n+1}}{(n+1)!} \begin{pmatrix} 0 \\ 1 \end{pmatrix} = \left(I_{2 \times 2} \times \frac{T}{2} + \frac{A_c T^2}{2} \right) \begin{pmatrix} 0 \\ 1 \end{pmatrix}$$

$$B_d(t=\frac{T}{2}) = \left(\begin{pmatrix} \frac{T}{2} & 0 \\ 0 & \frac{T}{2} \end{pmatrix} + \begin{pmatrix} 0 & 0.5 \\ 0 & 0 \end{pmatrix} \frac{T^2}{4} \right) \begin{pmatrix} 0 \\ 1 \end{pmatrix} = \begin{pmatrix} \frac{1}{8} T^2 \\ \frac{1}{2} T \end{pmatrix}$$

$$\begin{pmatrix} \begin{pmatrix} 1 & \frac{T}{2} \\ 0 & 1 \end{pmatrix} \begin{pmatrix} 1 & \frac{T}{2} \\ 0 & 1 \end{pmatrix} + \begin{pmatrix} \frac{1}{8} T^2 \\ \frac{1}{2} T \end{pmatrix} (k_1 \ k_2) & \begin{pmatrix} 1 & \frac{T}{2} \\ 0 & 1 \end{pmatrix} \begin{pmatrix} \frac{1}{8} T^2 \\ \frac{1}{2} T \end{pmatrix} \\ (k_1 \ k_2) & 0 \end{pmatrix}$$

$$= \begin{pmatrix} \begin{pmatrix} 1 & T \\ 0 & 1 \end{pmatrix} + \begin{pmatrix} \frac{1}{8} k_1 T^2 & \frac{1}{8} k_2 T^2 \\ \frac{1}{2} k_1 T & \frac{1}{2} k_2 T \end{pmatrix} & \begin{pmatrix} \frac{1}{8} T^2 + \frac{1}{4} T^2 \\ \frac{1}{2} T \end{pmatrix} \\ (k_1 \ k_2) & 0 \end{pmatrix}$$

$u(k)$ nicht kommt $u(k)$ kommt
wegen der Verzögerung

$$X(k) \quad X(k+\frac{1}{2}) \quad X(k+1)$$

benutzen
 $u(k-1)$